Coso

BracketAbstraction.Equality.fst
@@ -1,13 +1,188 @@
 module BracketAbstraction.Equality
 
 open SKI
+open SKI.Equality 
 open BracketAbstraction
+open Subst
+open Lam.Equality
 
 
-let subst_bracket (n i : nat) (t v : nclosed_lam n)
-: Lemma (requires i <= n) 
-        (ensures bracket_abstraction (subst_lam t v i) = subst (bracket_abstraction t) (bracket_abstraction v) i)
-= admit ()
+
+let abs_fnl (t : ski) : Lemma (fnl t ==> fnl (abstract_ski t))
+= ()
+
+
+let rec abstract_App (#n : nat) (t : nclosed_ski (n + 1)) (v : nclosed_ski n)
+: ski_eq #n (App (nclosed_abstraction (n + 1) t) v) (subst_nclosed_ski #n t v 0)
+= match t with
+  | App t u ->
+    let abs_t = nclosed_abstraction (n + 1) t  in
+    let abs_u = nclosed_abstraction (n + 1) u  in
+    let red_s = Red_S abs_t abs_u v in
+    let hi_t = abstract_App t v in
+    let hi_u = abstract_App u v in
+    let app_eq = App_eq hi_t hi_u in
+    Tran red_s app_eq
+  | Var 0 -> Red_I v
+  | Var j -> Red_K (Var (j - 1)) v
+  | S -> Red_K S v
+  | K -> Red_K K v
+  | I -> Red_K I v
+  | Unit -> Red_K Unit v
+
+
+let rec expand_subst (n : nat) (t : nclosed_ski (n + 1)) (v : nclosed_ski n)
+: Lemma (expand #n (subst_nclosed_ski t v 0) = subst_nclosed_ski (expand #(n + 1) t) (extend_ski #n #1 v) 0)
+= match t with
+  | App t u -> expand_subst n t v ; expand_subst n u v
+  | _ -> ()
+
+let rec subst_ski_eq (#n : nat) (#t #u: nclosed_ski (n + 1)) (eq : ski_eq t u)
+                     (v : nclosed_ski n)
+                     
+: Tot (ski_eq #n (subst_nclosed_ski t v 0) (subst_nclosed_ski u v 0))
+      (decreases eq)
+= let sub t = subst_nclosed_ski t v 0 in
+  match eq with
+  | Refl _ -> Refl _
+  | Symm eq -> Symm (subst_ski_eq eq v)
+  | Tran eq1 eq2 -> Tran (subst_ski_eq eq1 v) (subst_ski_eq eq2 v)
+  | App_eq eq1 eq2 -> App_eq (subst_ski_eq eq1 v) (subst_ski_eq eq2 v)
+  | Red_S f g x -> Red_S (sub f) (sub g) (sub x)
+  | Red_K x y -> Red_K (sub x) (sub y)
+  | Red_I x -> Red_I (sub x)
+  | Zeta eq ->
+    expand_subst n t v ;
+    expand_subst n u v ;
+    Zeta (subst_ski_eq #(n + 1) eq (extend_ski #n #1 v))
+
+
+
+let ( @ ) (#n : nat) (t u : nclosed_ski n) : nclosed_ski n = App t u
+
+
+let rec abstract_ski_eq (n : pos) (#t #u : nclosed_ski n) (t_eq_u : ski_eq t u)
+: Tot (ski_eq (nclosed_abstraction n t) (nclosed_abstraction n u))
+      (decreases t_eq_u)
+= match t_eq_u with
+| Red_S f g x -> admit ()
+// let f' : nclosed_ski n = extend_ski #(n - 1) #1 (nclosed_abstraction n f) in
+// let g' : nclosed_ski n = extend_ski #(n - 1) #1 (nclosed_abstraction n g) in
+// let x' : nclosed_ski n = extend_ski #(n - 1) #1 (nclosed_abstraction n x) in
+// let y : nclosed_ski n = Var (n - 1) in
+// let k  : nclosed_ski n = ((S @ ((S @ (K @ S)) @ f')) @ g') in 
+// let red_1 = Red_S k x' y in
+// let red_2 = Red_S (App (App S (App K S)) f') g' y in
+// let red_3 = Red_S (App K S) f' y in
+// let red_4 = Red_K S y in
+// let app_2 = App_eq red_2 (Refl (App x' y)) in
+// let app_3_1 = App_eq red_3 (Refl (App g' y)) in
+// let app_3_2 = App_eq app_3_1 (Refl (App x' y)) in
+// let app_4_1 = App_eq red_4 (Refl (App f' y)) in
+// let app_4_2 = App_eq app_4_1 (Refl (App g' y)) in 
+// let app_4_3 = App_eq app_4_2 (Refl (App x' y)) in
+// let red_5 = Red_S #n (App f' y) (App g' y) (App x' y) in
+// let lhs = Tran (Tran (Tran (Tran red_1 app_2) app_3_2) app_4_3) red_5 in
+// let red_1 = Red_S ((S @ f') @ x') ((S @ g') @ x') y in
+// let redl = Red_S f' x' y in
+// let redr = Red_S g' x' y in
+// let rhs = Tran red_1 (App_eq redl redr) in
+// assert (t = ((S @ f) @ g) @ x) ;
+// assert (abstract g = g') ;
+// Zeta (Tran lhs (Symm rhs))
+| Red_K x y ->
+let x' : nclosed_ski n = extend_ski #(n - 1) #1 (nclosed_abstraction n x) in
+let y' : nclosed_ski n = extend_ski #(n - 1) #1 (nclosed_abstraction n y) in
+let z : nclosed_ski n = Var (n - 1) in
+admit ()
+| Red_I x ->
+let x' : nclosed_ski n = extend_ski #(n - 1) #1 (nclosed_abstraction n x) in
+let y : nclosed_ski n = Var (n - 1) in
+let red_S = Red_S (K @ I) x' y in
+let red_K = Red_K I y in
+let app = App_eq (red_K) (Refl (x' @ y)) in
+let red_I = Red_I (x' @ y) in
+Zeta (Tran (Tran red_S app) red_I)
+| App_eq eq1 eq2 -> App_eq (App_eq (Refl S) (abstract_ski_eq n eq1)) (abstract_ski_eq n eq2)
+| Refl t -> Refl _
+| Symm eq -> Symm (abstract_ski_eq n eq)
+| Tran eq1 eq2 -> Tran (abstract_ski_eq n eq1) (abstract_ski_eq n eq2)
+| Zeta eq -> admit ()
+
+
+
+
+let rec shift_abs (n : nat) (t : ski)
+: Lemma (shiftn n (abstract t) = abstract (shiftn (n + 1) t))
+= match t with
+  | App t u -> shift_abs n t ; shift_abs n u 
+  | _ -> ()
+
+let rec shift_bracket (i : nat) (t : lam)
+: Lemma (ensures shiftn i (bracket_abstraction t) = bracket_abstraction (shiftn_lam i t))
+        (decreases t)
+= match t with
+  | Abs a t ->
+    shift_abs i (bracket_abstraction t) ;
+    shift_bracket (i + 1) t
+  | App t u -> shift_bracket i t ; shift_bracket i u
+  | _ -> ()
+
+let ski_eq_S_K (#n : nat) (t u : nclosed_ski n)
+: ski_eq #n (App (App S (App K t)) (App K u)) (App K (App t u))
+= let red_S = Red_S (extend_ski (App K t)) (extend_ski (App K u)) (Var n) in
+  let red_K_l = Red_K #(n + 1) (extend_ski t) (Var n) in
+  let red_K_r = Red_K #(n + 1) (extend_ski u) (Var n) in
+  let red_K_app = App_eq red_K_l red_K_r in
+  let lhs = Tran red_S red_K_app in
+  let red_K = Red_K #(n + 1) (extend_ski (App t u)) (Var n) in
+  let rhs = Symm red_K in
+  Zeta (Tran lhs rhs)
+
+let rec ski_eq_abstract (#n : nat) (t : nclosed_ski n)
+: ski_eq #n (nclosed_abstraction (n + 1) (shift_nclosed_ski t)) (App K t)
+= match t with
+  | App t u ->
+    let hi_t = ski_eq_abstract #n t in
+    let hi_u = ski_eq_abstract #n u in
+    let hi_appl = App_eq (Refl S) (hi_t) in
+    let hi_app = App_eq (hi_appl) (hi_u) in
+    let eq_SK = ski_eq_S_K #n t u in
+    Tran hi_app eq_SK
+  | _ -> Refl _
+
+let rec subst_abstract (#n : nat) (t : nclosed_ski (n + 2)) (v : nclosed_ski n) (i : nat {i <= n})
+: ski_eq #n (nclosed_abstraction (n + 1) (subst_nclosed_ski t (shift_nclosed_ski #n v) (i + 1)))
+            (subst_nclosed_ski (nclosed_abstraction (n + 2) t) v i)
+= match t with
+  | App t u ->
+    App_eq (App_eq (Refl S) (subst_abstract t v i)) (subst_abstract u v i)  
+  | Var j ->
+    if j = i + 1
+    then ski_eq_abstract #n v
+    else Refl _
+  | _ -> Refl _
+
+
+let rec subst_bracket (#n : nat) (t : nclosed_lam (n + 1)) (v : nclosed_lam n) (i : nat {i <= n})
+: Tot
+    (ski_eq #n
+      (nclosed_bracket_abstraction n (subst_nclosed_lam t v i))
+      (subst_nclosed_ski (nclosed_bracket_abstraction (n + 1) t) (nclosed_bracket_abstraction n v) i))
+    (decreases t)
+= match t with
+  | Abs _ t ->
+    // TODO comentar esto
+    shift_bracket 0 v ;
+    let hi = subst_bracket #(n + 1) t (shift_nclosed_lam v) (i + 1) in
+    let hi = abstract_ski_eq (n + 1) _ _ hi in 
+    let bracket_t = nclosed_bracket_abstraction (n + 2) t in
+    let bracket_v = nclosed_bracket_abstraction n v in
+    let subst_abstract_eq = subst_abstract bracket_t bracket_v i in
+    Tran hi subst_abstract_eq
+  | App t u -> App_eq (subst_bracket t v i) (subst_bracket u v i)
+  | _ -> Refl _
+
 
 let rec step_preserves_eq (#n : nat) (#t #u : nclosed_lam n) (st : step t u)
 : ski_eq #n (nclosed_bracket_abstraction n t) (nclosed_bracket_abstraction n u) =
@@ -15,10 +190,11 @@ let rec step_preserves_eq (#n : nat) (#t #u : nclosed_lam n) (st : step t u)
   | AppL st_t u -> 
     nclosed_step_impl n st ;
     App_eq (step_preserves_eq st_t) (Refl (nclosed_bracket_abstraction n u))
-  | Beta a t u ->
+  | AppR t st_u -> admit ()
+  | Beta _ t u ->
     nclosed_step_impl n st ;
-    match t with
-    | Var 0 -> Red_I (nclosed_bracket_abstraction n u)
-    | Abs _ t -> admit ()
-    | App t1 t2 -> admit ()
-    | _ -> admit ()
+    let bracket_t = nclosed_bracket_abstraction (n + 1) t in
+    let bracket_u = nclosed_bracket_abstraction n u in
+    Tran (abstract_App #n bracket_t bracket_u) (Symm (subst_bracket #n t u 0))
+  | Down _ st -> admit ()
+  
